VCVio/OracleComp/RunIO.lean
@@ -31,29 +31,20 @@ example : IO ℕ := do
   return (x * y)
 
 /-- Represent an `OracleComp` via the `IO` monad, allowing actual execution.
-Note that `OracleComp` as currently defined doesn't allow error messaging. -/
+NOTE: `OracleComp` as currently defined doesn't allow specialized error messaging.
+Changing this would just require adding a `String` to the `failure` constructor -/
 protected def runIO {α : Type} : ProbComp α → IO α
   | pure' α x => return x
   | queryBind' i _ α oa => do let u ← IO.rand 0 i; (oa u).runIO
   | failure' _ => throw (IO.userError "Computation failed during execution")
 
-private def lawLargeNumsTest (trials : ℕ) : IO Unit := do
-  let xs ← (replicate $[0..4] trials).runIO
-  IO.println ("Num 0s: " ++ toString (xs.1.1.count 0))
-  IO.println ("Num 1s: " ++ toString (xs.1.1.count 1))
-  IO.println ("Num 2s: " ++ toString (xs.1.1.count 2))
-  IO.println ("Num 3s: " ++ toString (xs.1.1.count 3))
-  IO.println ("Num 4s: " ++ toString (xs.1.1.count 4))
+private def lawLargeNumsTest (trials : ℕ) (die : ℕ) : IO Unit := do
+  let n : ℕ := trials * die
+  let xs ← (replicate n $[0..die - 1]).runIO
+  IO.println ("Rolling " ++ toString n ++ " " ++ toString die ++ "-sided dice:")
+  for i in List.range die do
+    IO.println <| "▸Num " ++ toString (i + 1) ++ "s: " ++ toString (xs.count i)
 
--- private def testOTP {n : ℕ} (m : Vector Bool n) : IO Unit := do
---   IO.println ("Initial Message: " ++ toString m.toList)
---   let k ← ((oneTimePad n).exec <| (oneTimePad n).keygen ()).runIO
---   IO.println ("Key: " ++ toString k.toList)
---   let σ ← ((oneTimePad n).exec <| (oneTimePad n).encrypt m k).runIO
---   IO.println ("Ciphertext: " ++ toString σ.toList)
---   let m' ← ((oneTimePad n).exec <| (oneTimePad n).decrypt σ k).runIO
---   IO.println ("Final Message: " ++ toString m'.toList)
-
--- #eval testOTP (Vector.replicate 100 true)
+#eval lawLargeNumsTest 100 6
 
 end OracleComp
